fv/lean/Ragu/Instances/Point/AddIncomplete.lean
@@ -68,17 +68,14 @@ def formal_instance : Core.Statements.FormalInstance where
   deserializeInput
   serializeOutput
 
-  Assumptions input :=
-    input.P1.isOnCurve Circuits.Point.Spec.EpAffineParams ∧ input.P2.isOnCurve Circuits.Point.Spec.EpAffineParams
-
   Spec input output :=
-    let ⟨P1, P2, nonzero⟩ := input
+    input.P1.isOnCurve Circuits.Point.Spec.EpAffineParams → input.P2.isOnCurve Circuits.Point.Spec.EpAffineParams →
     (
       -- If the x coordinates of P1 and P2 are different, then we can conclude that the
       -- addition output is affine and is the correct result of the addition
-      P1.x ≠ P2.x -> (
+      input.P1.x ≠ input.P2.x -> (
         (
-          match P1.add_incomplete P2  with
+          match input.P1.add_incomplete input.P2  with
           | none => False -- this case never happens
           | some res => output.P3 = res
         )
@@ -88,22 +85,22 @@ def formal_instance : Core.Statements.FormalInstance where
     (
       -- if the x coordinates of P1 and P2 are equal, then output nonzero is 0
       -- regardless of the input nonzero
-      (P1.x = P2.x -> output.nonzero = 0) ∧
+      (input.P1.x = input.P2.x -> output.nonzero = 0) ∧
 
       -- if the x coordinates of P1 and P2 are not equal, then output nonzero preserves
       -- non-zero-ness from input nonzero
-      (P1.x ≠ P2.x ->
-        (nonzero = 0 -> output.nonzero = 0) ∧
-        (nonzero ≠ 0 -> output.nonzero ≠ 0)
+      (input.P1.x ≠ input.P2.x ->
+        (input.nonzero = 0 -> output.nonzero = 0) ∧
+        (input.nonzero ≠ 0 -> output.nonzero ≠ 0)
       )
     )
 
+  reimplementation := Circuits.Point.AddIncomplete.circuit Circuits.Point.Spec.EpAffineParams 0
 
-  reimplementation := Circuits.Point.AddIncomplete.circuit Circuits.Point.Spec.EpAffineParams
-
-  same_circuit := by
+  same_constraints := by
     intro input
-    simp [Operations.toFlat, circuit_norm, FormalCircuit.toSubcircuit,
+    simp [Core.Statements.FlatOperation.eraseCompute, List.map,
+      Operations.toFlat, circuit_norm, GeneralFormalCircuit.toSubcircuit,
       deserializeInput, exportedOperations,
       Circuits.Point.AddIncomplete.circuit, Circuits.Point.AddIncomplete.elaborated, Circuits.Point.AddIncomplete.main,
       Circuits.Core.AllocMul.circuit, Circuits.Core.AllocMul.elaborated, Circuits.Core.AllocMul.main,
@@ -114,7 +111,7 @@ def formal_instance : Core.Statements.FormalInstance where
     constructor
   same_output := by
     intro input;
-    simp [circuit_norm, FormalCircuit.toSubcircuit,
+    simp [circuit_norm, GeneralFormalCircuit.toSubcircuit,
       deserializeInput, serializeOutput,
       Circuits.Point.AddIncomplete.circuit, Circuits.Point.AddIncomplete.elaborated, Circuits.Point.AddIncomplete.main,
       Circuits.Core.AllocMul.circuit, Circuits.Core.AllocMul.elaborated, Circuits.Core.AllocMul.main,
@@ -123,11 +120,18 @@ def formal_instance : Core.Statements.FormalInstance where
       Circuits.Element.Mul.circuit, Circuits.Element.Mul.elaborated, Circuits.Element.Mul.main]
     repeat (constructor <;> congr)
   same_spec := by
-    intro input output;
-    simp [Circuits.Point.AddIncomplete.circuit, Circuits.Point.AddIncomplete.Spec]
-    intro h1 h2
-    aesop
-  same_assumptions := by intro input; rfl
-
+    intro input output
+    constructor
+    · intro h h1 h2
+      generalize input.P1.add_incomplete input.P2 = d at h ⊢
+      cases d with
+      | none => exact h h1 h2
+      | some _ => exact h h1 h2
+    · intro h h1 h2
+      simp only [Circuits.Point.AddIncomplete.circuit, Circuits.Point.AddIncomplete.Spec] at h
+      generalize input.P1.add_incomplete input.P2 = d at h ⊢
+      cases d with
+      | none => exact h h1 h2
+      | some _ => exact h h1 h2
 
 end Ragu.Instances.Point.AddIncomplete
